strongInduction.v
@@ -1,0 +1,36 @@
+Require Import ssreflect ssrbool.
+Require Import Coq.Arith.Lt.
+Require Import Coq.Arith.PeanoNat.
+
+
+Theorem strong_induction:
+  forall P : nat -> Prop,
+    (forall n : nat, (forall k : nat, (k < n -> P k)) -> P n) ->
+    forall n : nat, P n.
+Proof.
+  intros.
+  apply H.
+  induction n ; intros.
+  + apply PeanoNat.Nat.nlt_0_r in H0 => //.
+  + move : (H n) => H1.
+    destruct k.
+    ++  destruct n.
+        +++ apply H1.
+            intros. apply PeanoNat.Nat.nlt_0_r in H2 => //.
+        +++ apply IHn.
+            apply PeanoNat.Nat.lt_0_succ.
+    ++ apply Lt.lt_S_n in H0.
+       apply H.
+       intros l H2.
+       apply IHn.
+       apply Lt.lt_n_Sm_le in H2.
+       apply (PeanoNat.Nat.le_lt_trans l k n) => //.
+Qed.
+
+
+(* Technical lemma that appears in proofs from time to time *)
+Lemma strong_induction_rewrite:
+  forall (P:nat -> Prop) n, (forall k : nat, S k <= S n -> P k) <-> (forall k : nat, k < S n -> P k).
+  intros.
+  split; intros; pose proof (Nat.lt_succ_r k n); eauto.
+Qed.
